Add a trivial equivalence checker for fun.

EquivalenceChecker.v
@@ -1,6 +1,6 @@
 From MyProject Require Export Expr.
 
-(* Complex equivalence checker *)
+(* Slightly more complex equivalence checker *)
 Fixpoint equivalence_checker (e1 e2 : expr) (s : state) : bool := 
   match e1, e2 with
     | Constant n1, Constant n2 => Nat.eqb n1 n2
@@ -8,5 +8,11 @@ Fixpoint equivalence_checker (e1 e2 : expr) (s : state) : bool :=
     | Plus e11 e12, Plus e21 e22 => andb (equivalence_checker e11 e21 s) (equivalence_checker e12 e22 s)
     | Minus e11 e12, Minus e21 e22 => andb (equivalence_checker e11 e21 s) (equivalence_checker e12 e22 s)
     | Mul e11 e12, Mul e21 e22 => andb (equivalence_checker e11 e21 s) (equivalence_checker e12 e22 s)
+    | _, _ => false
+  end.
+
+Definition trivial_equivalence_checker (e1 e2 : expr) (s : state) : bool := 
+  match e1, e2 with
+    | Constant n1, Constant n2 => Nat.eqb n1 n2
     | _, _ => false
   end.
