Main.v
@@ -4,17 +4,12 @@ From Coq Require Import Strings.String.
 Open Scope string_scope.
 From MyProject Require Export EquivalenceChecker.
 
-
-(* TODO: Write an SMT-based equivalence checker here. *)
-(* And prove it equivalent in the same way ... *)
-
-
 (* destruct and induction both generate the same number of goals:
      one for each data constructor,
      the difference is induction generates additional inductive hypothesis
      for the recursive data constructors (like Plus, Mul, MInus)*)
 Lemma one_more_lemma (e1 e2 : expr)  (s : state) :
-  EquivalenceChecker.equivalence_checker e1 e2 s = true -> e1 = e2.
+  equivalence_checker e1 e2 s = true -> e1 = e2.
   Proof. (* intro is one term, intros is multiple terms *)
     intros H. (* Stuff on the right hand side of the colon doesn't go automatically into environment or context*)
     (* TODO: Need a more general induction hypothesis here .*)
@@ -109,6 +104,18 @@ Lemma lemma1 :
       reflexivity.
 Qed.
 
+Lemma trivial_lemma1 :
+  forall (e1 e2 : expr) (s : state), trivial_equivalence_checker e1 e2 s = true -> e1 = e2.
+  Proof.
+    intros e1 e2 s.
+    unfold trivial_equivalence_checker.
+    destruct e1, e2; try discriminate.
+    - intros H.
+      apply Nat.eqb_eq in H.
+      rewrite H.
+      reflexivity.
+  Qed.
+
 (* Prove that the equivalence checker is correct *)
 Theorem equivalence_checker_correct:
   forall (e1 e2 : expr) (s : state), equivalence_checker e1 e2 s = true -> aequiv e1 e2 s.
@@ -120,6 +127,18 @@ intros H.
 apply lemma1 in H.
 rewrite H.
 reflexivity.
+Qed.
+
+(* Prove that trivial equivalence checker is correct *)
+Theorem trivial_equivalence_checker_correct:
+  forall (e1 e2 : expr) (s : state), trivial_equivalence_checker e1 e2 s = true -> aequiv e1 e2 s.
+Proof.
+  intros e1 e2 s.
+  unfold aequiv.
+  intros H.
+  apply trivial_lemma1 in H.
+  rewrite H.
+  reflexivity.
 Qed.
 
 (* A*(B+C) = AB + AC *)
