SmtEquivalenceChecker.v
@@ -1,0 +1,2 @@
+(* TODO: Write an SMT-based equivalence checker here. *)
+(* And prove it equivalent in the same way ... *)
